platform/Scheduler.v
@@ -3,173 +3,7 @@ Require Import AutoSep Bags Malloc Queue.
 Set Implicit Arguments.
 
 
-Section starL.
-  Variable A : Type.
-  Variable P : A -> HProp.
-
-  Open Scope Sep_scope.
-
-  Fixpoint starL (ls : list A) : HProp :=
-    match ls with
-      | nil => Emp
-      | x :: ls => P x * starL ls
-    end.
-End starL.
-
-Section starB.
-  Definition bagify (ls : list (W * W)) : bag :=
-    fold_left add ls empty.
-
-  Definition predB := W * W -> HProp.
-  Variable P : predB.
-
-  Open Scope Sep_scope.
-
-  Definition starB (b : bag) : HProp :=
-    Ex ls, [| b %= bagify ls |] * starL P ls.
-
-  Ltac to_himp := repeat intro.
-  Ltac from_himp := match goal with
-                      | [ |- interp ?specs (?p ?x ?y ---> ?q ?x ?y) ] =>
-                        generalize dependent y; generalize dependent x; generalize dependent specs;
-                          change (p ===> q)
-                    end.
-
-  Theorem starB_empty_bwd : Emp ===> starB empty.
-    to_himp; apply existsR with nil; from_himp; sepLemma.
-  Qed.
-
-  Lemma exists_starL_fwd : forall A (P : A -> _) Q,
-    (Ex x, P x) * Q ===> Ex x, P x * Q.
-    sepLemma.
-  Qed.
-
-  Lemma equiv_symm : forall b1 b2,
-    b1 %= b2
-    -> b2 %= b1.
-    unfold equiv; firstorder.
-  Qed.
-
-  Lemma equiv_trans : forall b1 b2 b3,
-    b1 %= b2
-    -> b2 %= b3
-    -> b1 %= b3.
-    unfold equiv; firstorder.
-  Qed.
-
-  Lemma bagify_cong : forall ls b1 b2,
-    b1 %= b2
-    -> fold_left add ls b1 %= fold_left add ls b2.
-    induction ls; simpl; intuition.
-  Qed.
-
-  Lemma add_something : forall v ls b,
-    fold_left add ls (b %+ v) %= fold_left add ls b %+ v.
-    induction ls; simpl; intuition.
-    eapply equiv_trans; [ | apply IHls ].
-    apply bagify_cong; auto.
-  Qed.
-
-  Theorem starB_add_bwd : forall b v, starB b * P v ===> starB (b %+ v).
-    intros; eapply Himp_trans; [ apply exists_starL_fwd | ]; cbv beta.
-    to_himp; apply existsL; intro ls; apply existsR with (v :: ls); from_himp.
-    simpl; generalize (starL P ls); generalize (P v); sepLemma.
-    unfold bagify in *; simpl.
-    apply equiv_symm; eapply equiv_trans; [ apply add_something | ]; auto.
-  Qed.
-
-  Lemma exists_starR_bwd : forall P A (Q : A -> _),
-    Ex x, P * Q x ===> P * (Ex x, Q x).
-    sepLemma.
-  Qed.
-
-  Fixpoint nuke (p : W * W) (ls : list (W * W)) : list (W * W) :=
-    match ls with
-      | nil => nil
-      | p' :: ls => if W_W_dec p p' then ls else p' :: nuke p ls
-    end.
-
-  Lemma starL_del_fwd : forall v ls, In v ls
-    -> starL P ls ===> P v * starL P (nuke v ls).
-    induction ls; unfold bagify in *; simpl in *; intuition subst.
-    destruct (W_W_dec v v); apply Himp_refl || tauto.
-    destruct (W_W_dec v (a0, b)); subst; try apply Himp_refl.
-    simpl.
-    eapply Himp_trans.
-    apply Himp_star_frame; [ apply Himp_refl | apply H ].
-    generalize (starL P (nuke v ls)); generalize (P (a0, b)); generalize (P v); sepLemma.
-  Qed.
-
-  Lemma del_something : forall v ls b,
-    v %in b
-    -> fold_left add ls (b %- v) %= fold_left add ls b %- v.
-    induction ls; simpl; intuition.
-    eapply equiv_trans; [ | apply IHls ].
-    apply bagify_cong; auto.
-    auto.
-  Qed.
-
-  Lemma bagify_nuke' : forall v ls, In v ls
-    -> forall b, fold_left add (nuke v ls) b %= fold_left add ls b %- v.
-    induction ls; simpl; intuition subst.
-    destruct (W_W_dec v v); intuition.
-    eapply equiv_trans; [ | apply del_something ].
-    apply bagify_cong; auto.
-    auto.
-    destruct (W_W_dec v (a0, b)); subst.
-    eapply equiv_trans; [ | apply del_something ].
-    apply bagify_cong; auto.
-    auto.
-    simpl; auto.
-  Qed.
-
-  Lemma bagify_nuke : forall v ls, In v ls
-    -> bagify (nuke v ls) %= bagify ls %- v.
-    intros; apply bagify_nuke'; auto.
-  Qed.
-
-  Lemma bagify_In' : forall v ls b b',
-    v %in b
-    -> b %= fold_left add ls b'
-    -> In v ls \/ v %in b'.
-    unfold bagify; induction ls; simpl; intuition.
-    eapply IHls in H; [ | eauto ].
-    intuition (eauto; bags).
-  Qed.
-
-  Lemma bagify_In : forall v ls b,
-    v %in b
-    -> b %= bagify ls
-    -> In v ls.
-    intros.
-    eapply bagify_In' in H0; eauto.
-    intuition bags.
-  Qed.    
-
-  Hint Resolve bagify_In bagify_nuke.
-
-  Theorem starB_del_fwd : forall b v, v %in b
-    -> starB b ===> P v * starB (b %- v).
-    intros; eapply Himp_trans; [ | apply exists_starR_bwd ]; cbv beta.
-    to_himp; apply existsL; intro ls; apply existsR with (nuke v ls).
-    specialize (starL_del_fwd v ls);
-      generalize (starL P ls); generalize (P v); generalize (starL P (nuke v ls)).
-    intros; from_himp.
-    sepLemma.
-    eapply equiv_trans; [ | apply equiv_symm; apply bagify_nuke ].
-    auto.
-    eauto.
-    transitivity (h0 * h); eauto.
-    sepLemma.
-  Qed.
-End starB.
-
-
-(** * The actual scheduler (will later move above stuff to Bags) *)
-
 (* What does it mean for a program counter to be valid for a suspended thread? *)
-
-Notation "#5" := (fun x => Lift (Lift (Lift (Lift (Lift (Var0 x)))))) : PropX_scope.
 
 Definition susp (sc pc sp : W) : HProp := fun s m =>
   (ExX (* pre *) : settings * state, Cptr pc #0
@@ -193,12 +27,6 @@ Inductive mergeSusp : Prop := MS.
 Inductive splitSusp : Prop := SS.
 
 Hint Constructors mergeSusp splitSusp.
-
-Definition any : HProp := fun _ _ => [| True |]%PropX.
-
-Theorem any_easy : forall P, P ===> any.
-  unfold any; repeat intro; step auto_ext; auto.
-Qed.
 
 Module Type SCHED.
   Parameter susps : bag -> W -> HProp.
@@ -323,15 +151,6 @@ Definition m := bimport [[ "malloc"!"malloc" @ [mallocS],
 
 Local Hint Extern 1 (@eq W _ _) => words.
 
-Lemma propToWord_elim_not1 : forall P b,
-  P \is b
-  -> b <> 1
-  -> ~P.
-  bags.
-Qed.
-
-Local Hint Immediate propToWord_elim_not1.
-
 Lemma susp_elim : forall specs sc pc sp P stn st,
   interp specs (![ susp sc pc sp * P ] (stn, st))
   -> exists pre, specs pc = Some pre
@@ -362,18 +181,6 @@ Lemma susp_elim : forall specs sc pc sp P stn st,
   repeat apply himp_star_frame; try reflexivity.
   instantiate (1 := fun p => fr_exit (fst p) (snd p)); reflexivity.
   eauto.
-
-  Theorem substH_lift5 : forall p' t1 t2 t3 t4 t5 p,
-    substH (lift (t1 :: t2 :: t3 :: t4 :: t5 :: nil) p') p = lift (t1 :: t2 :: t3 :: t4 :: nil) p'.
-    reflexivity.
-  Qed.
-
-  Theorem substH_lift6 : forall p' t1 t2 t3 t4 t5 t6 p,
-    substH (lift (t1 :: t2 :: t3 :: t4 :: t5 :: t6 :: nil) p') p = lift (t1 :: t2 :: t3 :: t4 :: t5 :: nil) p'.
-    reflexivity.
-  Qed.
-
-  Hint Rewrite substH_lift5 substH_lift6 : sepFormula.
   post.
   rewrite sepFormula_eq; propxFo; eauto.
 Qed.
@@ -422,24 +229,6 @@ Theorem ok : moduleOk m.
 
   post; evaluate hints.
 
-  (* Within [H], find a conjunct [P] such that [which P] doesn't fail, and reassociate [H]
-   * to put [P] in front. *)
-  Ltac toFront which H :=
-    let rec toFront' P k :=
-      match P with
-        | SEP.ST.star ?Q ?R =>
-          toFront' Q ltac:(fun it P' => k it (SEP.ST.star P' R))
-          || toFront' R ltac:(fun it P' => k it (SEP.ST.star P' Q))
-            || fail 2
-        | _ => which P; k P (@SEP.ST.emp W (settings * state) nil)
-      end in
-      match type of H with
-        | interp ?specs (![ ?P ] ?st) => toFront' P ltac:(fun it P' =>
-          let H' := fresh in
-            assert (H' : interp specs (![ SEP.ST.star it P' ] st)) by step auto_ext;
-              clear H; rename H' into H)
-      end.
-
   toFront ltac:(fun P => match P with
                            | susp _ _ _ => idtac
                          end) H8.
@@ -456,7 +245,6 @@ Theorem ok : moduleOk m.
   descend; step hints.
   apply any_easy.
 
-  Show Existentials.
   unfold localsInvariant; simpl.
   intros.
   step auto_ext.
