src/PropX.v
@@ -1570,6 +1570,7 @@ Notation "#1" := (fun x => Lift (Var0 x)) : PropX_scope.
 Notation "#2" := (fun x => Lift (Lift (Var0 x))) : PropX_scope.
 Notation "#3" := (fun x => Lift (Lift (Lift (Var0 x)))) : PropX_scope.
 Notation "#4" := (fun x => Lift (Lift (Lift (Lift (Var0 x))))) : PropX_scope.
+Notation "#5" := (fun x => Lift (Lift (Lift (Lift (Lift (Var0 x)))))) : PropX_scope.
 
 Delimit Scope PropX_scope with PropX.
 Bind Scope PropX_scope with PropX propX.
